implemented pretty printing for RISC-V

RiscvDialect/RISCV64/Base.lean
@@ -7,88 +7,117 @@ open RV64Semantics /- access the semantics -/
 
 namespace RISCV64
 /-! ## The `RISCV64` dialect -/
+
 /-!
 ## Dialect operation definitions
 Modelled operations such that their inputs arguments are up to two register content values. Any other attributes e.g flags
 are encoded as part of the op-code.
 
- Modells base ISA & ZBA/ZBB extension instructions.
+We modell the RV64I base instruction set: https://github.com/riscv/riscv-isa-manual/blob/main/src/rv64.adoc, therefore allow for an 64-bit address space.
+And operations out of selected RISC-V extension:
+    - `M`: stadnart integer division and multiplication instruction extension
+
+    - `B`: extension for Bit manipulation (comprises instructions provided by the `Zba`, `Zbb`, and `Zbs` extensions)
+            here: https://github.com/riscv/riscv-isa-manual/blob/main/src/b-st-ext.adoc
+
+    - `Zicond` : extension for conditional operations https://github.com/riscvarchive/riscv-zicond/blob/main/zicondops.adoc
 -/
-inductive Op
-|const : (val : Int) → Op -- const is not part of the RISC-V ISA but is used to in this dialect to modell immediates.
-|addiw (imm : BitVec 12) -- TO DO: rethink this design
-|lui (imm : BitVec 20)
-|auipc (imm : BitVec 20)
-|slliw (shamt : BitVec 5)
-|srliw (shamt : BitVec 5)
-|sraiw (shamt : BitVec 5)
-|slli (shamt : BitVec 6)
-|srli (shamt : BitVec 6)
-|srai (shamt : BitVec 6)
-|addw
-|subw
-|sllw
-|srlw
-|sraw
-|add
-|slt
-|sltu
-|and
-|or
-|xor
-|sll
-|srl
-|sub
-|sra
-|remw
-|rem
-|mul
-|mulu
-|mulw
-|mulh
-|mulhu
-|mulhsu
-|divu
-|rol
-|ror
-|remwu
-|remu
- --the sign or unsigned when calling the function -> pattern match on to mul op to get the correct cases
-|divw
-|divwu
-|div
-|addi (imm : BitVec 12)
-|slti (imm : BitVec 12)
-|sltiu (imm : BitVec 12)
-|andi (imm : BitVec 12)
-|ori (imm : BitVec 12)
-|xori (imm : BitVec 12)
-|czero.eqz
-|czero.nez
-|bclr
-|bext
-|binv
-|bset
-|bclri (shamt : BitVec 6)
-|bexti (shamt : BitVec 6)
-|binvi (shamt : BitVec 6)
-|bseti (shamt : BitVec 6)
-|sext.b
-|sext.h
-|zext.h
-|rolw
-|rorw
-/-
-|pack
-|packh
--- TO DO zbb_rytpe full
+inductive Op -- ! whenever add an operation, extend the pretty EDSL accordingly !
+|   const : (val : Int) → Op -- const is not part of the RISC-V ISA but is used to in this dialect to modell immediates.
+-- `RV64I` base ISA instructions (integer add, subtract & logical operations)
+|  lui (imm : BitVec 20)
+|  auipc (imm : BitVec 20)
+|  addi (imm : BitVec 12)
+|  andi (imm : BitVec 12)
+|  ori (imm : BitVec 12)
+|  xori (imm : BitVec 12)
+|  addiw (imm : BitVec 12)
+|  add
+|  slli (shamt : BitVec 6)
+|  sub
+|  and
+|  or
+|  xor
+|  sll
+|  srl
+|  sra
+|  addw
+|  subw
+|  sllw
+|  srlw
+|  sraw
+-- fence
+|  slti (imm : BitVec 12)
+|  sltiu (imm : BitVec 12)
+|  srli (shamt : BitVec 6)
+|  srai (shamt : BitVec 6)
+|  slliw (shamt : BitVec 5)
+|  srliw (shamt : BitVec 5)
+|  sraiw (shamt : BitVec 5)
+|  slt
+|  sltu
+-- RISC-V `M` extension instructions (multiply& divide)
+| mul    -- performs signed multiplication on 64 x 64 bits and returns the lower 64 bits of the result .
+| mulu   -- performs unsigned multiplication on 64 x 64 bits and returns the lower 64 bits of the result .
+| mulw
+| mulh   -- performs signed multiplication on 64 x 64 bits and returns the upper 64 bits of the result.
+| mulhu  -- performs unsigned multiplication on 64 x 64 bits and returns the upper 64 bits of the result.
+| mulhsu -- performs multiplication on (rs1 signed) x (rs2 unsigned) and returns the upper 64 bits of the result.
+| divw
+| divwu
+| div    -- signed division
+| divu   -- unsigned division
+| remw
+| rem    --sign of result is according to sign of dividend
+| remwu
+| remu
+-- RISC-V `Zba` extension
 |add.uw
 |sh1add.uw
 |sh2add.uw
 |sh3add.uw
 |sh1add
 |sh2add
-|sh3add -/
+|sh3add
+-- slli.uw missing
+-- part of the RISC-V `Zbb` & `Zbkb` extension
+| rol
+| ror
+| rolw
+| rorw
+| sext.b
+| sext.h
+| zext.h
+/-
+|pack
+|packh
+-/
+-- part of the RISC-V `Zbs` extension
+| bclr
+| bclri (shamt : BitVec 6)
+| bext
+| bexti (shamt : BitVec 6)
+| binv
+| binvi (shamt : BitVec 6)
+| bset
+| bseti (shamt : BitVec 6)
+/- RISC-V `Zicond` conditional operations extension  -/
+| czero.eqz -- returns zero, if the condition rs2 is equal to zero, else rs1.
+| czero.nez -- returns zero, if the condition rs2 is non-zero, else rs1.
+
+/-
+TO DO zbb_rytpe full -> will be implementeed as soon as MVP exists.
+| andn
+| orn
+| xnor
+| max
+| maxu
+| min
+| minu
+| rol --> done
+| ror --> done
+-/
+
 deriving DecidableEq, Repr
 
 
@@ -98,25 +127,20 @@ Defining a type system for the `RISCV64` dialect. `bv` represents bit vector.
 -/
 inductive Ty
   | bv : Ty
-  deriving DecidableEq, Repr
+  deriving DecidableEq, Repr, Inhabited
 
 /-!
 Connecting the `bv` type to its underlying Lean type `BitVec 64`. By providing a `TyDenote` instance,
 we define how the `RISCV64` types transalte into actual Lean types.
 -/
-open TyDenote (toType) in
-instance RV64TyDenote : TyDenote Ty where
+
+instance : TyDenote Ty where
 toType := fun
 | Ty.bv => BitVec 64
 
-/--
-Provding a default instance for `bv`, which is a 64-bit zero bit vector.
--/
-instance : Inhabited (TyDenote.toType (t : Ty)) where
-  default := by
-    cases t
-    exact (0#64)
-
+instance (ty : Ty) : Inhabited (TyDenote.toType ty) where
+  default := match ty with
+    | .bv  => 0#64
 
 /--
 ## Dialect operation definitions
@@ -131,69 +155,75 @@ encounters a `sig` it can replace it by its definition.
 
 @[simp, reducible]
 def Op.sig : Op → List Ty
-  |.const _ =>  []
-  |.mulu  => [Ty.bv, Ty.bv]
-  |mulh  => [Ty.bv, Ty.bv]
-  |mulhu  => [Ty.bv, Ty.bv]
-  |mulhsu  => [Ty.bv, Ty.bv]
-  |divu =>  [Ty.bv, Ty.bv]
-  |rol => [Ty.bv, Ty.bv]
-  |ror => [Ty.bv, Ty.bv]
-  |.remwu  => [Ty.bv, Ty.bv]
-  |.remu  =>  [Ty.bv, Ty.bv]
-  |.addiw (imm : BitVec 12) => [Ty.bv]
-  |.lui (imm : BitVec 20) => [Ty.bv]
-  |.auipc (imm : BitVec 20)  => [Ty.bv]
-  |.slliw (shamt : BitVec 5)  => [Ty.bv]
-  |.srliw (shamt : BitVec 5) => [Ty.bv]
-  |.sraiw (shamt : BitVec 5) => [Ty.bv]
-  |.slli (shamt : BitVec 6) => [Ty.bv]
-  |.srli (shamt : BitVec 6) => [Ty.bv]
-  |srai (shamt : BitVec 6) => [Ty.bv]
-  |.addw => [Ty.bv, Ty.bv]
-  |.subw => [Ty.bv, Ty.bv]
-  |.sllw => [Ty.bv, Ty.bv]
-  |.srlw => [Ty.bv, Ty.bv]
-  |.sraw => [Ty.bv, Ty.bv]
-  |.add => [Ty.bv, Ty.bv]
-  |.slt => [Ty.bv, Ty.bv]
-  |.sltu => [Ty.bv, Ty.bv]
-  |.and => [Ty.bv, Ty.bv]
-  |.or => [Ty.bv, Ty.bv]
-  |.xor => [Ty.bv, Ty.bv]
-  |.sll => [Ty.bv, Ty.bv]
-  |.srl => [Ty.bv, Ty.bv]
-  |.sub => [Ty.bv, Ty.bv]
-  |.sra => [Ty.bv, Ty.bv]
-  |.remw  => [Ty.bv, Ty.bv]
-  |.rem  =>  [Ty.bv, Ty.bv]
-  |.mul => [Ty.bv, Ty.bv]
-  |.mulw => [Ty.bv, Ty.bv]
-  |.div  =>  [Ty.bv, Ty.bv]
-  |.divw  =>  [Ty.bv, Ty.bv]
-  |.divwu  =>  [Ty.bv, Ty.bv]
-  |.addi (imm : BitVec 12) => [Ty.bv]
-  |.slti (imm : BitVec 12) => [Ty.bv]
-  |.sltiu (imm : BitVec 12) => [Ty.bv]
-  |.andi (imm : BitVec 12) => [Ty.bv]
-  |.ori (imm : BitVec 12) => [Ty.bv]
-  |.xori (imm : BitVec 12) => [Ty.bv]
-  |.czero.eqz =>  [Ty.bv, Ty.bv]
-  |.czero.nez =>  [Ty.bv, Ty.bv]
-  |.sext.b => [Ty.bv]
-  |.sext.h => [Ty.bv]
-  |.zext.h => [Ty.bv]
-  |bclr => [Ty.bv, Ty.bv]
-  |bext => [Ty.bv, Ty.bv]
-  |binv => [Ty.bv, Ty.bv]
-  |bset  => [Ty.bv, Ty.bv]
-  |bclri (shamt : BitVec 6) => [Ty.bv]
-  |bexti (shamt : BitVec 6) => [Ty.bv]
-  |binvi (shamt : BitVec 6) => [Ty.bv]
-  |bseti (shamt : BitVec 6) => [Ty.bv]
-  |rolw => [Ty.bv, Ty.bv]
-  |rorw => [Ty.bv, Ty.bv]
-
+  | .const _ =>  []
+  | .mulu  => [Ty.bv, Ty.bv]
+  | .mulh  => [Ty.bv, Ty.bv]
+  | .mulhu  => [Ty.bv, Ty.bv]
+  | .mulhsu  => [Ty.bv, Ty.bv]
+  | .divu =>  [Ty.bv, Ty.bv]
+  | .rol => [Ty.bv, Ty.bv]
+  | .ror => [Ty.bv, Ty.bv]
+  | .remwu  => [Ty.bv, Ty.bv]
+  | .remu  =>  [Ty.bv, Ty.bv]
+  | .addiw (imm : BitVec 12) => [Ty.bv]
+  | .lui (imm : BitVec 20) => [Ty.bv]
+  | .auipc (imm : BitVec 20)  => [Ty.bv]
+  | .slliw (shamt : BitVec 5)  => [Ty.bv]
+  | .srliw (shamt : BitVec 5) => [Ty.bv]
+  | .sraiw (shamt : BitVec 5) => [Ty.bv]
+  | .slli (shamt : BitVec 6) => [Ty.bv]
+  | .srli (shamt : BitVec 6) => [Ty.bv]
+  | .srai (shamt : BitVec 6) => [Ty.bv]
+  | .addw => [Ty.bv, Ty.bv]
+  | .subw => [Ty.bv, Ty.bv]
+  | .sllw => [Ty.bv, Ty.bv]
+  | .srlw => [Ty.bv, Ty.bv]
+  | .sraw => [Ty.bv, Ty.bv]
+  | .add => [Ty.bv, Ty.bv]
+  | .slt => [Ty.bv, Ty.bv]
+  | .sltu => [Ty.bv, Ty.bv]
+  | .and => [Ty.bv, Ty.bv]
+  | .or => [Ty.bv, Ty.bv]
+  | .xor => [Ty.bv, Ty.bv]
+  | .sll => [Ty.bv, Ty.bv]
+  | .srl => [Ty.bv, Ty.bv]
+  | .sub => [Ty.bv, Ty.bv]
+  | .sra => [Ty.bv, Ty.bv]
+  | .remw  => [Ty.bv, Ty.bv]
+  | .rem  =>  [Ty.bv, Ty.bv]
+  | .mul => [Ty.bv, Ty.bv]
+  | .mulw => [Ty.bv, Ty.bv]
+  | .div  =>  [Ty.bv, Ty.bv]
+  | .divw  =>  [Ty.bv, Ty.bv]
+  | .divwu  =>  [Ty.bv, Ty.bv]
+  | .addi (imm : BitVec 12) => [Ty.bv]
+  | .slti (imm : BitVec 12) => [Ty.bv]
+  | .sltiu (imm : BitVec 12) => [Ty.bv]
+  | .andi (imm : BitVec 12) => [Ty.bv]
+  | .ori (imm : BitVec 12) => [Ty.bv]
+  | .xori (imm : BitVec 12) => [Ty.bv]
+  | .czero.eqz =>  [Ty.bv, Ty.bv]
+  | .czero.nez =>  [Ty.bv, Ty.bv]
+  | .sext.b => [Ty.bv]
+  | .sext.h => [Ty.bv]
+  | .zext.h => [Ty.bv]
+  | .bclr => [Ty.bv, Ty.bv]
+  | .bext => [Ty.bv, Ty.bv]
+  | .binv => [Ty.bv, Ty.bv]
+  | .bset  => [Ty.bv, Ty.bv]
+  | .bclri (shamt : BitVec 6) => [Ty.bv]
+  | .bexti (shamt : BitVec 6) => [Ty.bv]
+  | .binvi (shamt : BitVec 6) => [Ty.bv]
+  | .bseti (shamt : BitVec 6) => [Ty.bv]
+  | .rolw => [Ty.bv, Ty.bv]
+  | .rorw => [Ty.bv, Ty.bv]
+  | .add.uw => [Ty.bv, Ty.bv]
+  | .sh1add.uw => [Ty.bv, Ty.bv]
+  | .sh2add.uw => [Ty.bv, Ty.bv]
+  | .sh3add.uw => [Ty.bv, Ty.bv]
+  | .sh1add => [Ty.bv, Ty.bv]
+  | .sh2add => [Ty.bv, Ty.bv]
+  | .sh3add => [Ty.bv, Ty.bv]
 
 /--
 Specifing the `outTy` of each `RISCV64` operation.
@@ -254,33 +284,42 @@ def Op.outTy : Op  → Ty
   |.sext.b => Ty.bv
   |.sext.h => Ty.bv
   |.zext.h => Ty.bv
-  |bclr => Ty.bv
-  |bext => Ty.bv
-  |binv => Ty.bv
-  |bset  => Ty.bv
-  |bclri (shamt : BitVec 6) => Ty.bv
-  |bexti (shamt : BitVec 6) => Ty.bv
-  |binvi (shamt : BitVec 6) => Ty.bv
-  |bseti (shamt : BitVec 6) => Ty.bv
-  |rolw => Ty.bv
-  |rorw => Ty.bv
+  |.bclr => Ty.bv
+  |.bext => Ty.bv
+  |.binv => Ty.bv
+  |.bset  => Ty.bv
+  |.bclri (shamt : BitVec 6) => Ty.bv
+  |.bexti (shamt : BitVec 6) => Ty.bv
+  |.binvi (shamt : BitVec 6) => Ty.bv
+  |.bseti (shamt : BitVec 6) => Ty.bv
+  |.rolw => Ty.bv
+  |.rorw => Ty.bv
+  | .add.uw => Ty.bv
+  | .sh1add.uw => Ty.bv
+  | .sh2add.uw => Ty.bv
+  | .sh3add.uw => Ty.bv
+  | .sh1add => Ty.bv
+  | .sh2add => Ty.bv
+  | .sh3add => Ty.bv
 
 
 /-- Combine `outTy` and `sig` together into a `Signature`. -/
 @[simp, reducible]
 def Op.signature : Op → Signature (Ty) :=
-  fun o => {sig := Op.sig o, outTy := Op.outTy o, regSig := []} --ASK what is meant by regSig ?
-
+  fun o => {sig := Op.sig o, outTy := Op.outTy o, regSig := []}
 
 
 /--
 Bundling the `Ops`and `Ty`into a dialect and abbreviating `RISCV64` into a dialect named `RV64`.
 We pass our `Op.signature` as an instance -/
+@[simp]
 abbrev RV64 : Dialect where
   Op := Op
   Ty := Ty
 
 instance : DialectSignature RV64 := ⟨Op.signature⟩
+
+
 
 -- DEBUG: only addapted the get0 get1 of the instruction that where used in the insteuction selcetion so far, to be extended
 -- I assume the layout is add (then all the args in the op code) (then args in the signature) ret_val
@@ -307,60 +346,67 @@ instance : DialectDenote (RV64) where
   |.slli shamt, regs, _  => SHIFTIOP_pure64_RISCV_SLLI shamt (regs.getN 0 (by simp [DialectSignature.sig, signature]))
   |.srli shamt, regs, _  => SHIFTIOP_pure64_RISCV_SRLI shamt (regs.getN 0 (by simp [DialectSignature.sig, signature]))
   |.srai shamt, regs, _  => SHIFTIOP_pure64_RISCV_SRAI shamt  (regs.getN 0 (by simp [DialectSignature.sig, signature]))
-  |.addw, regs, _  =>  RTYPEW_pure64_RISCV_ADDW (regs.getN 0 (by simp [DialectSignature.sig, signature]))  (regs.getN 1 (by simp [DialectSignature.sig, signature]))
-  |.subw, regs, _  => RTYPEW_pure64_RISCV_SUBW (regs.getN 0 (by simp [DialectSignature.sig, signature]))  (regs.getN 1 (by simp [DialectSignature.sig, signature]))
-  |.sllw, regs, _  => RTYPEW_pure64_RISCV_SLLW (regs.getN 0 (by simp [DialectSignature.sig, signature]))  (regs.getN 1 (by simp [DialectSignature.sig, signature]))
-  |.srlw, regs, _  => RTYPEW_pure64_RISCV_SRLW (regs.getN 0 (by simp [DialectSignature.sig, signature]))  (regs.getN 1 (by simp [DialectSignature.sig, signature]))
-  |.sraw, regs, _ => RTYPEW_pure64_RISCV_SRAW (regs.getN 0 (by simp [DialectSignature.sig, signature]))  (regs.getN 1 (by simp [DialectSignature.sig, signature]))
-  |.add, regs, _ => RTYPE_pure64_RISCV_ADD (regs.getN 0 (by simp [DialectSignature.sig, signature]))  (regs.getN 1 (by simp [DialectSignature.sig, signature]))
-  |.slt, regs, _ => RTYPE_pure64_RISCV_SLT (regs.getN 0 (by simp [DialectSignature.sig, signature]))  (regs.getN 1 (by simp [DialectSignature.sig, signature]))
-  |.sltu, regs, _ => RTYPE_pure64_RISCV_SLTU (regs.getN 0 (by simp [DialectSignature.sig, signature]))  (regs.getN 1 (by simp [DialectSignature.sig, signature]))
-  |.and, regs, _ => RTYPE_pure64_RISCV_AND (regs.getN 0 (by simp [DialectSignature.sig, signature]))  (regs.getN 1 (by simp [DialectSignature.sig, signature]))
-  |.or, regs, _ => RTYPE_pure64_RISCV_OR (regs.getN 0 (by simp [DialectSignature.sig, signature]))  (regs.getN 1 (by simp [DialectSignature.sig, signature]))
-  |.xor, regs, _ => RTYPE_pure64_RISCV_XOR (regs.getN 0 (by simp [DialectSignature.sig, signature]))  (regs.getN 1 (by simp [DialectSignature.sig, signature]))
+  -- The semantics are defined such that the first argument is the 2nd operand. see Semantics.lean
+  |.addw, regs, _  =>  RTYPEW_pure64_RISCV_ADDW (regs.getN 1 (by simp [DialectSignature.sig, signature]))  (regs.getN 0 (by simp [DialectSignature.sig, signature]))
+  |.subw, regs, _  => RTYPEW_pure64_RISCV_SUBW (regs.getN 1 (by simp [DialectSignature.sig, signature]))  (regs.getN 0 (by simp [DialectSignature.sig, signature]))
+  |.sllw, regs, _  => RTYPEW_pure64_RISCV_SLLW (regs.getN 1 (by simp [DialectSignature.sig, signature]))  (regs.getN 0 (by simp [DialectSignature.sig, signature]))
+  |.srlw, regs, _  => RTYPEW_pure64_RISCV_SRLW (regs.getN 1 (by simp [DialectSignature.sig, signature]))  (regs.getN 0 (by simp [DialectSignature.sig, signature]))
+  |.sraw, regs, _ => RTYPEW_pure64_RISCV_SRAW (regs.getN 1 (by simp [DialectSignature.sig, signature]))  (regs.getN 0 (by simp [DialectSignature.sig, signature]))
+  |.add, regs, _ => RTYPE_pure64_RISCV_ADD (regs.getN 1 (by simp [DialectSignature.sig, signature]))  (regs.getN 0 (by simp [DialectSignature.sig, signature]))
+  |.slt, regs, _ => RTYPE_pure64_RISCV_SLT (regs.getN 1 (by simp [DialectSignature.sig, signature]))  (regs.getN 0 (by simp [DialectSignature.sig, signature]))
+  |.sltu, regs, _ => RTYPE_pure64_RISCV_SLTU (regs.getN 1 (by simp [DialectSignature.sig, signature]))  (regs.getN 0 (by simp [DialectSignature.sig, signature]))
+  |.and, regs, _ => RTYPE_pure64_RISCV_AND (regs.getN 1 (by simp [DialectSignature.sig, signature]))  (regs.getN 0 (by simp [DialectSignature.sig, signature]))
+  |.or, regs, _ => RTYPE_pure64_RISCV_OR (regs.getN 1 (by simp [DialectSignature.sig, signature]))  (regs.getN 0 (by simp [DialectSignature.sig, signature]))
+  |.xor, regs, _ => RTYPE_pure64_RISCV_XOR (regs.getN 1 (by simp [DialectSignature.sig, signature]))  (regs.getN 0 (by simp [DialectSignature.sig, signature]))
   |.sll, regs, _ => RTYPE_pure64_RISCV_SLL (regs.getN 1 (by simp [DialectSignature.sig, signature]))  (regs.getN 0 (by simp [DialectSignature.sig, signature]))
   |.srl, regs, _ => RTYPE_pure64_RISCV_SRL (regs.getN 1 (by simp [DialectSignature.sig, signature]))  (regs.getN 0 (by simp [DialectSignature.sig, signature]))
-  |.sub, regs, _  => RTYPE_pure64_RISCV_SUB (regs.getN 0 (by simp [DialectSignature.sig, signature]))  (regs.getN 1 (by simp [DialectSignature.sig, signature]))
+  |.sub, regs, _  => RTYPE_pure64_RISCV_SUB (regs.getN 1 (by simp [DialectSignature.sig, signature]))  (regs.getN 0 (by simp [DialectSignature.sig, signature]))
   |.sra, regs, _  => RTYPE_pure64_RISCV_SRA (regs.getN 1 (by simp [DialectSignature.sig, signature]))  (regs.getN 0 (by simp [DialectSignature.sig, signature]))
-  |.remw, regs, _  => REMW_pure64_signed (regs.getN 0 (by simp [DialectSignature.sig, signature]))  (regs.getN 1 (by simp [DialectSignature.sig, signature]))-- double-check
-  |.remwu, regs, _  => REMW_pure64_unsigned (regs.getN 0 (by simp [DialectSignature.sig, signature]))  (regs.getN 1 (by simp [DialectSignature.sig, signature]))-- double-check
+  |.remw, regs, _  => REMW_pure64_signed (regs.getN 1 (by simp [DialectSignature.sig, signature]))  (regs.getN 0 (by simp [DialectSignature.sig, signature]))
+  |.remwu, regs, _  => REMW_pure64_unsigned (regs.getN 1 (by simp [DialectSignature.sig, signature]))  (regs.getN 0 (by simp [DialectSignature.sig, signature]))
   |.rem, regs, _  =>  REM_pure64_signed (regs.getN 1 (by simp [DialectSignature.sig, signature]))  (regs.getN 0 (by simp [DialectSignature.sig, signature]))
   |.remu, regs, _ =>  REM_pure64_unsigned (regs.getN 1 (by simp [DialectSignature.sig, signature]))  (regs.getN 0 (by simp [DialectSignature.sig, signature]))
-  |.mulu, regs, _ => MUL_pure64_fff (regs.getN 0 (by simp [DialectSignature.sig, signature]))  (regs.getN 1 (by simp [DialectSignature.sig, signature])) -- double check
-  --|.mul false false true , regs, _ => RV64.MUL_pure64_fft (regs.getN 0 (by simp [DialectSignature.sig, signature]))  (regs.getN 1 (by simp [DialectSignature.sig, signature]))
-  --|.mul  false true false , regs, _ => RV64.MUL_pure64_ftf (regs.getN 0 (by simp [DialectSignature.sig, signature]))  (regs.getN 1 (by simp [DialectSignature.sig, signature]))
-  |.mulhu,regs, _ => MUL_pure64_tff (regs.getN 0 (by simp [DialectSignature.sig, signature]))  (regs.getN 1 (by simp [DialectSignature.sig, signature]))
-  |.mul ,regs, _ => MUL_pure64_ftt (regs.getN 0 (by simp [DialectSignature.sig, signature]))  (regs.getN 1 (by simp [DialectSignature.sig, signature]))
-  --|.mul  true false true,regs, _ => RV64.MUL_pure64_tft (regs.getN 0 (by simp [DialectSignature.sig, signature]))  (regs.getN 1 (by simp [DialectSignature.sig, signature]))
-  |.mulhsu ,regs, _ => MUL_pure64_ttf (regs.getN 0 (by simp [DialectSignature.sig, signature]))  (regs.getN 1 (by simp [DialectSignature.sig, signature]))
-  |.mulh,regs, _ => MUL_pure64_ttt (regs.getN 0 (by simp [DialectSignature.sig, signature]))  (regs.getN 1 (by simp [DialectSignature.sig, signature]))
-  |.mulw,  regs, _ => MULW_pure64 (regs.getN 0 (by simp [DialectSignature.sig, signature]))  (regs.getN 1 (by simp [DialectSignature.sig, signature])) -- double check
+  |.mulu, regs, _ => MUL_pure64_fff (regs.getN 1 (by simp [DialectSignature.sig, signature]))  (regs.getN 0 (by simp [DialectSignature.sig, signature])) -- double check
+  --|.mul false false true , regs, _ => RV64.MUL_pure64_fft (regs.getN 0 (by simp [DialectSignature.sig, signature]))  (regs.getN 1 (by simp [DialectSignature.sig, signature])) :: no corresponding RISC-V exists
+  --|.mul  false true false , regs, _ => RV64.MUL_pure64_ftf (regs.getN 0 (by simp [DialectSignature.sig, signature]))  (regs.getN 1 (by simp [DialectSignature.sig, signature])) :: no corresponding RISC-V exists
+  |.mulhu,regs, _ => MUL_pure64_tff (regs.getN 1 (by simp [DialectSignature.sig, signature]))  (regs.getN 0 (by simp [DialectSignature.sig, signature]))
+  |.mul ,regs, _ => MUL_pure64_ftt (regs.getN 1 (by simp [DialectSignature.sig, signature]))  (regs.getN 0 (by simp [DialectSignature.sig, signature]))
+  --|.mul  true false true,regs, _ => RV64.MUL_pure64_tft (regs.getN 0 (by simp [DialectSignature.sig, signature]))  (regs.getN 1 (by simp [DialectSignature.sig, signature])) :: no corresponding RISC-V exists
+  |.mulhsu ,regs, _ => MUL_pure64_ttf (regs.getN 1 (by simp [DialectSignature.sig, signature]))  (regs.getN 0 (by simp [DialectSignature.sig, signature]))
+  |.mulh,regs, _ => MUL_pure64_ttt (regs.getN 1 (by simp [DialectSignature.sig, signature]))  (regs.getN 0 (by simp [DialectSignature.sig, signature]))
+  |.mulw,  regs, _ => MULW_pure64 (regs.getN 1 (by simp [DialectSignature.sig, signature]))  (regs.getN 0 (by simp [DialectSignature.sig, signature])) -- double check
   |.div, regs, _  =>  DIV_pure64_signed (regs.getN 1 (by simp [DialectSignature.sig, signature]))  (regs.getN 0 (by simp [DialectSignature.sig, signature]))
-  |.divu,  regs, _ =>  DIV_pure64_unsigned (regs.getN 0 (by simp [DialectSignature.sig, signature]))  (regs.getN 1 (by simp [DialectSignature.sig, signature]))
-  |.divw, regs, _  =>  DIVW_pure64_signed (regs.getN 0 (by simp [DialectSignature.sig, signature]))  (regs.getN 1 (by simp [DialectSignature.sig, signature]))
-  |.divwu, regs, _ =>  DIVW_pure64_unsigned (regs.getN 0 (by simp [DialectSignature.sig, signature]))  (regs.getN 1 (by simp [DialectSignature.sig, signature]))
+  |.divu,  regs, _ =>  DIV_pure64_unsigned (regs.getN 1 (by simp [DialectSignature.sig, signature]))  (regs.getN 0 (by simp [DialectSignature.sig, signature]))
+  |.divw, regs, _  =>  DIVW_pure64_signed (regs.getN 1 (by simp [DialectSignature.sig, signature]))  (regs.getN 0 (by simp [DialectSignature.sig, signature]))
+  |.divwu, regs, _ =>  DIVW_pure64_unsigned (regs.getN 1 (by simp [DialectSignature.sig, signature]))  (regs.getN 0 (by simp [DialectSignature.sig, signature]))
   |.addi imm, reg, _  => ITYPE_pure64_RISCV_ADDI  imm (reg.getN 0 (by simp [DialectSignature.sig, signature]))
   |.slti imm, reg, _  => ITYPE_pure64_RISCV_SLTI  imm (reg.getN 0 (by simp [DialectSignature.sig, signature]))
   |.sltiu imm, reg, _ => ITYPE_pure64_RISCV_SLTIU  imm (reg.getN 0 (by simp [DialectSignature.sig, signature]))
   |.andi imm, reg, _=> ITYPE_pure64_RISCV_ANDI  imm (reg.getN 0 (by simp [DialectSignature.sig, signature]))
   |.ori imm, reg, _ => ITYPE_pure64_RISCV_ORI  imm (reg.getN 0 (by simp [DialectSignature.sig, signature]))
   |.xori imm, reg, _=> ITYPE_pure64_RISCV_XORI  imm (reg.getN 0 (by simp [DialectSignature.sig, signature]))
-  |.czero.eqz, regs, _ => ZICOND_RTYPE_pure64_RISCV_CZERO_EQZ (regs.getN 0 (by simp [DialectSignature.sig, signature]))  (regs.getN 1 (by simp [DialectSignature.sig, signature]))
-  |.czero.nez, regs, _ => ZICOND_RTYPE_pure64_RISCV_RISCV_CZERO_NEZ (regs.getN 0 (by simp [DialectSignature.sig, signature]))  (regs.getN 1 (by simp [DialectSignature.sig, signature]))
+  |.czero.eqz, regs, _ => ZICOND_RTYPE_pure64_RISCV_CZERO_EQZ (regs.getN 1 (by simp [DialectSignature.sig, signature]))  (regs.getN 0 (by simp [DialectSignature.sig, signature]))
+  |.czero.nez, regs, _ => ZICOND_RTYPE_pure64_RISCV_RISCV_CZERO_NEZ (regs.getN 1 (by simp [DialectSignature.sig, signature]))  (regs.getN 0 (by simp [DialectSignature.sig, signature]))
   |.sext.b, reg, _ => ZBB_EXTOP_pure64_RISCV_SEXTB (reg.getN 0 (by simp [DialectSignature.sig, signature]))
   |.sext.h, reg, _ => ZBB_EXTOP_pure64_RISCV_SEXTH (reg.getN 0 (by simp [DialectSignature.sig, signature]))
   |.zext.h, reg, _ => ZBB_EXTOP_pure64_RISCV_ZEXTH (reg.getN 0 (by simp [DialectSignature.sig, signature]))
-  |.bclr, regs, _  => ZBS_RTYPE_pure64_RISCV_BCLR (regs.getN 0 (by simp [DialectSignature.sig, signature]))  (regs.getN 1 (by simp [DialectSignature.sig, signature]))
-  |.bext, regs, _  => ZBS_RTYPE_pure64_RISCV_BEXT (regs.getN 0 (by simp [DialectSignature.sig, signature]))  (regs.getN 1 (by simp [DialectSignature.sig, signature]))
-  |.binv, regs, _  => ZBS_RTYPE_pure64_BINV (regs.getN 0 (by simp [DialectSignature.sig, signature]))  (regs.getN 1 (by simp [DialectSignature.sig, signature]))
-  |.bset, regs, _   => ZBS_RTYPE_pure64_RISCV_BSET (regs.getN 0 (by simp [DialectSignature.sig, signature]))  (regs.getN 1 (by simp [DialectSignature.sig, signature]))
+  |.bclr, regs, _  => ZBS_RTYPE_pure64_RISCV_BCLR (regs.getN 1 (by simp [DialectSignature.sig, signature]))  (regs.getN 0 (by simp [DialectSignature.sig, signature]))
+  |.bext, regs, _  => ZBS_RTYPE_pure64_RISCV_BEXT (regs.getN 1 (by simp [DialectSignature.sig, signature]))  (regs.getN 0 (by simp [DialectSignature.sig, signature]))
+  |.binv, regs, _  => ZBS_RTYPE_pure64_BINV (regs.getN 1 (by simp [DialectSignature.sig, signature]))  (regs.getN 0 (by simp [DialectSignature.sig, signature]))
+  |.bset, regs, _   => ZBS_RTYPE_pure64_RISCV_BSET (regs.getN 1 (by simp [DialectSignature.sig, signature]))  (regs.getN 0 (by simp [DialectSignature.sig, signature]))
   |.bclri shamt , reg, _  => ZBS_IOP_pure64_RISCV_BCLRI (shamt) (reg.getN 0 (by simp [DialectSignature.sig, signature]))
   |.bexti shamt, reg, _  => ZBS_IOP_pure64_RISCV_BEXTI (shamt) (reg.getN 0 (by simp [DialectSignature.sig, signature]))
   |.binvi shamt, reg, _ => ZBS_IOP_pure64_RISCV_BINVI (shamt) (reg.getN 0 (by simp [DialectSignature.sig, signature]))
   |.bseti shamt, reg, _ => ZBS_IOP_pure64_RISCV_BSETI (shamt) (reg.getN 0 (by simp [DialectSignature.sig, signature]))
-  |.rolw, regs, _ => ZBB_RTYPEW_pure64_RISCV_ROLW (regs.getN 0 (by simp [DialectSignature.sig, signature]))  (regs.getN 1 (by simp [DialectSignature.sig, signature]))
-  |.rorw, regs, _ => ZBB_RTYPEW_pure64_RISCV_RORW (regs.getN 0 (by simp [DialectSignature.sig, signature]))  (regs.getN 1 (by simp [DialectSignature.sig, signature]))
-  |.rol, regs, _ => ZBB_RTYPE_pure64_RISCV_ROL (regs.getN 0 (by simp [DialectSignature.sig, signature]))  (regs.getN 1 (by simp [DialectSignature.sig, signature]))
-  |.ror, regs, _ => ZBB_RTYPE_pure64_RISCV_ROR (regs.getN 0 (by simp [DialectSignature.sig, signature]))  (regs.getN 1 (by simp [DialectSignature.sig, signature]))
-
+  |.rolw, regs, _ => ZBB_RTYPEW_pure64_RISCV_ROLW (regs.getN 1 (by simp [DialectSignature.sig, signature]))  (regs.getN 0 (by simp [DialectSignature.sig, signature]))
+  |.rorw, regs, _ => ZBB_RTYPEW_pure64_RISCV_RORW (regs.getN 1 (by simp [DialectSignature.sig, signature]))  (regs.getN 0 (by simp [DialectSignature.sig, signature]))
+  |.rol, regs, _ => ZBB_RTYPE_pure64_RISCV_ROL (regs.getN 1 (by simp [DialectSignature.sig, signature]))  (regs.getN 0 (by simp [DialectSignature.sig, signature]))
+  |.ror, regs, _ => ZBB_RTYPE_pure64_RISCV_ROR (regs.getN 1 (by simp [DialectSignature.sig, signature]))  (regs.getN 0 (by simp [DialectSignature.sig, signature]))
+  | .add.uw, regs, _  =>  ZBA_RTYPEUW_pure64_RISCV_ADDUW (regs.getN 1 (by simp [DialectSignature.sig, signature]))  (regs.getN 0 (by simp [DialectSignature.sig, signature]))
+  | .sh1add.uw , regs, _  =>  ZBA_RTYPEUW_pure64_RISCV_SH1ADDUW (regs.getN 1 (by simp [DialectSignature.sig, signature]))  (regs.getN 0 (by simp [DialectSignature.sig, signature]))
+  | .sh2add.uw, regs, _  =>  ZBA_RTYPEUW_pure64_RISCV_SH2ADDUW (regs.getN 1 (by simp [DialectSignature.sig, signature]))  (regs.getN 0 (by simp [DialectSignature.sig, signature]))
+  | .sh3add.uw, regs, _  =>  ZBA_RTYPEUW_pure64_RISCV_SH3ADDUW (regs.getN 1 (by simp [DialectSignature.sig, signature]))  (regs.getN 0 (by simp [DialectSignature.sig, signature]))
+  | .sh1add, regs, _  =>  ZBA_RTYPE_pure64_RISCV_SH1ADD (regs.getN 1 (by simp [DialectSignature.sig, signature]))  (regs.getN 0 (by simp [DialectSignature.sig, signature]))
+  | .sh2add, regs, _  =>  ZBA_RTYPE_pure64_RISCV_SH2ADD (regs.getN 1 (by simp [DialectSignature.sig, signature]))  (regs.getN 0 (by simp [DialectSignature.sig, signature]))
+  | .sh3add, regs, _  =>  ZBA_RTYPE_pure64_RISCV_SH3ADD (regs.getN 1 (by simp [DialectSignature.sig, signature]))  (regs.getN 0 (by simp [DialectSignature.sig, signature]))
 end RISCV64
