RiscvDialect/RISCV64/Semantics.lean
@@ -167,6 +167,11 @@ def MULW_pure64 (rs2_val : (BitVec 64)) (rs1_val : (BitVec 64)) : BitVec 64 :=
         (BitVec.ofInt 65
           ((BitVec.extractLsb 31 0 rs1_val).toInt * (BitVec.extractLsb 31 0 rs2_val).toInt).toNat)))
 
+/-!
+## mul operations flags
+ the suffix indicates how the flags are assumed to be set.
+{ high := _, signed_rs1:= _, signed_rs2 := _  }
+-/
 def MUL_pure64_fff (rs2_val : BitVec 64) (rs1_val : BitVec 64) : BitVec 64 :=
      BitVec.extractLsb 63 0
         (BitVec.extractLsb' 0 128 (BitVec.ofInt 129 (max (Int.mul (Int.ofNat rs1_val.toNat) (Int.ofNat rs2_val.toNat)) 0)))
@@ -350,17 +355,36 @@ BitVec.signExtend 64
  def ZBB_RTYPE_pure64_RISCV_ROR (rs2_val : BitVec 64) (rs1_val : BitVec 64) :=
       BitVec.or (BitVec.ushiftRight rs1_val (BitVec.extractLsb 5 0 rs2_val).toNat)
     (BitVec.shiftLeft rs1_val ((BitVec.extractLsb' 0 6 (BitVec.ofInt (7) (64)) - BitVec.extractLsb 5 0 rs2_val)).toNat)
+
+ def ZBA_RTYPEUW_pure64_RISCV_ADDUW (rs2_val : BitVec 64) (rs1_val : BitVec 64) :=
+      BitVec.zeroExtend 64 (BitVec.extractLsb 31 0 rs1_val) <<< 0#2 + rs2_val
+
+
+def  ZBA_RTYPEUW_pure64_RISCV_SH1ADDUW (rs2_val : BitVec 64) (rs1_val : BitVec 64) :=
+    BitVec.add (BitVec.zeroExtend (Int.toNat 64) (BitVec.extractLsb 31 0 rs1_val) <<< 1#2)  (rs2_val)
+
+def ZBA_RTYPEUW_pure64_RISCV_SH2ADDUW (rs2_val : BitVec 64) (rs1_val : BitVec 64) :=
+      BitVec.add (BitVec.zeroExtend (Int.toNat 64) (BitVec.extractLsb 31 0 rs1_val) <<< 2#2) rs2_val
+
+def  ZBA_RTYPEUW_pure64_RISCV_SH3ADDUW (rs2_val : BitVec 64) (rs1_val : BitVec 64) :=
+      BitVec.add (BitVec.zeroExtend (Int.toNat 64) (BitVec.extractLsb 31 0 rs1_val) <<< 3#2)  rs2_val
+
+def ZBA_RTYPE_pure64_RISCV_SH1ADD (rs2_val : BitVec 64) (rs1_val : BitVec 64) :=
+    BitVec.add (rs1_val <<< 1#2) rs2_val
+
+def ZBA_RTYPE_pure64_RISCV_SH2ADD (rs2_val : BitVec 64) (rs1_val : BitVec 64) :=
+    BitVec.add (rs1_val <<< 2#2) rs2_val
+
+def ZBA_RTYPE_pure64_RISCV_SH3ADD(rs2_val : BitVec 64) (rs1_val : BitVec 64) :=
+    BitVec.add (rs1_val <<< 3#2) rs2_val
+
 /-
-|binv
-|bset
-|bclri
-|bexti
-|binvi
-|bseti
-|sext.b
-|sext.h
-|zext.h
-|rolw
-|rorw
--/
+to complete in the future:
+def ZBB_RYTPE_pure64_RISCV_ + rytpe from sail side is missing.
+|pack
+|packh
+slli.uw
+
+ -/
+
 end RV64Semantics
