RiscvDialect/RISCV64/all.lean
@@ -1,3 +1,4 @@
 import RiscvDialect.RISCV64.Syntax
 import RiscvDialect.RISCV64.Base
 import RiscvDialect.RISCV64.Semantics
+import RiscvDialect.RISCV64.PrettyEDSL
