thesis_examples/background/rfl_by_rfl.lean
@@ -1,0 +1,9 @@
+/--
+
+(ty_eq : ty = DialectSignature.outTy op)
+to proof this we can either pass `rfl`object or a proof `by rfl`
+This is the diffrence between term and tactic mode.
+Either directly provide an element of the type or advise Lean in `tactic mode`
+how to construct the corresponding term
+
+-/
